\documentclass{article}
\usepackage{amsmath}

\begin{document}
$$
\log P(S) = \int_R f(y) dy 
$$$$
\frac{\partial}{\partial \theta} \log P(s) 
= \frac{\partial}{\partial\theta} \log \int_R \varphi(y;\theta,\Sigma) dy 
= \frac{1}{P(S)} \frac{\partial}{\partial \theta} P(S)
$$

$$
\frac{\partial}{\partial\theta} P(S) = \int_R \left(\Sigma^{-1}y - \Sigma^{-1}\theta \right)  \varphi(y;\theta, \Sigma)dy
$$$$
= P(S) \left(\Sigma^{-1}E(y|S) - \Sigma^{-1} \theta \right)
$$$$
\Rightarrow \frac{\partial}{\partial \theta} \log P(s)  = \Sigma^{-1}E(y|S) - \Sigma^{-1} \theta
$$

$$
\frac{\partial^{2}}{\partial\theta^{2}} \log P(S) = 
-\Sigma^{-1} + \frac{\partial}{\partial\theta} \Sigma^{-1} E(y|S)
$$

$$
\frac{\partial}{\partial\theta} E(y|S) =
\int_R \frac{y}{P(S)^{2}}\left(P(S) (\Sigma^{-1} y - \Sigma^{-1}\theta) \varphi(y;\theta,\Sigma) -\varphi(y; \theta,\Sigma) P(S)(\Sigma^{-1}E(y|S) -\Sigma^{-1}\theta)
\right)
$$$$
=\int_R f(y|S) y\left(\Sigma^{-1}y - \Sigma^{-1} E(y|S) \right)dy = Var(y|S)\Sigma^{-1}
$$

$$
\Rightarrow \frac{\partial^{2}}{\partial\theta^{2}} \log P(S) 
= Var(\Sigma^{-1}y|S) - \Sigma^{-1}
$$





\end{document}