\documentclass{article}

\usepackage{amsmath, amssymb}

\begin{document}

\section{GLMER E-Step}
$$
P(Z_i= 1 | y, \theta) = 
\frac{\int \prod_{j} f(y_{ij}|X,\beta_1) g(v)dv}
{\int \prod_{j} f(y_{ij}|X,\beta_1) f(v)dv + \int \prod_{j} f(y_{ij}|X,\beta_0) g(v)dv}
$$

$$
\approx \frac{\sum_{m=1}^{M} \frac{g(v)}{\tilde{g}_1(v)}\prod_{j} f(y_{ij}|X,\beta_1,v_{m})}
{\sum_{m=1}^{M} \frac{g(v)}{\tilde{g}_1(v)}\prod_{j} f(y_{ij}|X,\beta_1,v_{m}) + 
\frac{g(v)}{\tilde{g}_0(v)}\prod_{j} f(y_{ij}|X,\beta_0,v_{m})}
$$$$
= \left(
1 + \frac{\sum_{m=1}^{M} \frac{g(v)}{\tilde{g}_0(v)} \prod_{j} f(y_{ij}|X,\beta_0,v_{m})}
{\sum_{m=1}^{M}\frac{g(v)}{\tilde{g}_1(v)}\prod_{j} f(y_{ij}|X,\beta_1,v_{m})}
\right)^{-1}
$$





\break
\section{Some Computation}

$$
\mathcal{L(\theta)} = \int \prod_{k=1}^{K} f_\theta(x_k, v) \pi(v)dv
$$$$
l(\theta) = \log\int \prod_{k=1}^{K} f_\theta(x_k, v) \pi(v)dv
$$$$
\frac{\partial}{\partial \theta} l(\theta) = \frac{1}{\mathcal{L(\theta)}}
\int \frac{\partial}{\partial \theta} \prod_{k=1}^{K} f_\theta(x_k) \pi(v)dv
$$$$
 = \frac{1}{\mathcal{L(\theta)}}
\int \prod_{k=1}^{K} f_\theta(x_k, v)
\left( \sum_{k=1}^{K} \frac{\partial}{\partial\theta} \log f_\theta(x_k, v) \right)
\pi(v)dv
$$

$$
\approx \left(\sum_{j=1}^{J}  \prod_{k=1}^{K} f_\theta(x_k, v_j)\right)^{-1}
\left(\sum_{j=1}^{J} \prod_{k=1}^{K} f_\theta(x_k, v_j)
\left( \sum_{k=1}^{K} \frac{\partial}{\partial\theta} \log f_\theta(x_k, v_j) \right)\right)
$$


\break
\section{Constrained Random Effect}
$$
\min\frac{1}{2}\sum_{i=1}^{n} \sum_{k=1}^{K} \sum_{j=1}^{J} w_{ijk}(x_{ijk} - \hat{\mu}_{ik})^{2}
$$$$
w_{ik} := \sum_{j} w_{ijk}
$$$$
s.t. \; \sum_{i}w_{ik} \mu_{ik} = 0 \;\; \forall k
$$

For a set $k$:
$$
L_k = \frac{1}{2}\sum_i\sum_j w_{ij} (x_{ij} - \hat{\mu}_{i})^{2} + \lambda\sum_{i} w_{i} \hat\mu_{i}
$$

Solve a system of equations:
$$
-\sum_{j} w_{ij} (x_{ij} - \hat{\mu}_i) + \lambda w_i  = 0 \;\;\;\;\; \forall i 
$$$$
\sum_i w_i \hat\mu_i = 0
$$$$
\Rightarrow \lambda = \frac{\sum_{ij} w_{ij} x_{ij}}{\sum_{i} w_i }
$$$$
\Rightarrow \hat\mu_i 
= \frac{\sum_{j} w_{ij} x_{ij} - \lambda w_i}{w_i}
= \frac{\sum_{j} w_{ij} x_{ij}}{\sum_{j} w_{ij}} - \lambda := \bar{x}_i - \bar{\mu}
$$







\end{document}

